GroupApproximation.lean
@@ -27,7 +27,6 @@ import GroupApproximation.Monsters.CyclicBaseCalibration
 import GroupApproximation.Monsters.LiteralCyclicCalibration
 import GroupApproximation.Sofic.LiteralNonMFLinearWitness
 import GroupApproximation.Sofic.LiteralNonMFEndpoint
-import GroupApproximation.Sofic.ConceptualNonMFProof
 import GroupApproximation.Sofic.LiteralBaseTranslationLattice
 import GroupApproximation.Sofic.LiteralBaseP13Replay
 import GroupApproximation.Sofic.LiteralBasePropertyTBridge
